src/lib/state/DY.Lib.State.Typed.fst
@@ -75,6 +75,23 @@ val state_was_set:
 let state_was_set #a #ls tr prin sess_id content =
   tagged_state_was_set tr ls.tag prin sess_id (serialize _ content)
 
+val state_was_set_grows:
+  #a:Type -> {|lsa:local_state a|} ->
+  tr1:trace -> tr2:trace -> 
+  prin:principal -> sess_id:state_id -> content:a ->
+  Lemma
+  (requires tr1 <$ tr2
+    /\ state_was_set tr1 prin sess_id content
+  )
+  (ensures
+    state_was_set tr2 prin sess_id content
+  )
+  [SMTPat (state_was_set #a #lsa tr1 prin sess_id content); SMTPat (tr1 <$ tr2)]
+let state_was_set_grows #a #ls tr1 tr2 prin sess_id content  = 
+  reveal_opaque (`%state_was_set) (state_was_set #a);
+  tagged_state_was_set_grows tr1 tr2 ls.tag prin sess_id (serialize _ content)
+
+
 [@@ "opaque_to_smt"]
 val set_state:
   #a:Type -> {|local_state a|} ->
@@ -133,6 +150,7 @@ val get_state_invariant:
       | None -> True
       | Some content -> (
         spred.pred tr prin sess_id content
+        /\ state_was_set tr prin sess_id content
       )
     )
   ))
@@ -141,6 +159,12 @@ val get_state_invariant:
    SMTPat (has_local_state_predicate spred)]
 let get_state_invariant #a #ls #invs spred prin sess_id tr =
   reveal_opaque (`%get_state) (get_state #a)
+  ; match get_tagged_state ls.tag prin sess_id tr with
+  | (None, _) -> ()
+  | (Some content, _) -> (
+        serialize_parse_inv_lemma #bytes a content
+       ;reveal_opaque (`%state_was_set) (state_was_set #a)
+  )
 
 val state_was_set_implies_pred:
   #a:Type -> {|local_state a|} ->
@@ -161,3 +185,5 @@ val state_was_set_implies_pred:
 let state_was_set_implies_pred #a #ls #invs tr spred prin sess_id content =
   parse_serialize_inv_lemma #bytes a content;
   reveal_opaque (`%state_was_set) (state_was_set #a)
+
+
